thys/First_Order_Terms/Lists_are_Infinite.thy
@@ -3,7 +3,7 @@ Author:  Christian Sternagel <c.sternagel@gmail.com>
 Author:  René Thiemann <rene.thiemann@uibk.ac.at>
 License: LGPL
 *)
-subsection \<open>Make lists instances of the infinite-class and some further lemmas on lists.\<close>
+subsection \<open>Make lists instances of the infinite-class\<close>
 
 theory Lists_are_Infinite
   imports Fresh_Identifiers.Fresh
@@ -11,15 +11,5 @@ begin
 
 instance list :: (type) infinite
   by (intro_classes, rule infinite_UNIV_listI)
-
-lemma upt_append_upt: "i \<le> j \<Longrightarrow> j \<le> k \<Longrightarrow> [i..<j] @ [j..<k] = [i..<k]"
-  using upt_add_eq_append[of i j "k - j"] by auto
-
-lemma split_list_index: assumes "i < length xs"
-  shows "xs = map ((!) xs) [0..<i] @ xs ! i # map ((!) xs) [Suc i..<length xs]"
-  using assms
-  by (metis list.map(2) map_append map_nth nat_less_le
-      upt_append_upt upt_conv_Cons zero_order(1))
-
 
 end
